feat: Adding a storage option to the KeyStore (#594)
The key store now allows for both a default DynamoDB table,
or any custom storage system.

The important aspect about the key store
is the fact that branch keys can be versioned easily,
and are cryptographically safe to use.
The actual storage medium is not important.

See: https://github.com/awslabs/aws-encryption-sdk-specification/blob/master/changes/2024-6-17_key-store-persistance/background.md#background

AwsCryptographicMaterialProviders/runtimes/python/src/aws_cryptographic_material_providers/smithygenerated/aws_cryptography_keystore/references.py
@@ -1,0 +1,447 @@
+# Copyright Amazon.com Inc. or its affiliates. All Rights Reserved.
+# SPDX-License-Identifier: Apache-2.0
+# Do not modify this file. This file is machine generated, and any changes to it will be overwritten.
+
+import abc
+import aws_cryptographic_material_providers.internaldafny.generated.AwsCryptographyKeyStoreTypes
+from aws_cryptographic_material_providers.internaldafny.generated.AwsCryptographyKeyStoreTypes import (
+    GetEncryptedActiveBranchKeyInput_GetEncryptedActiveBranchKeyInput as DafnyGetEncryptedActiveBranchKeyInput,
+    GetEncryptedActiveBranchKeyOutput_GetEncryptedActiveBranchKeyOutput as DafnyGetEncryptedActiveBranchKeyOutput,
+    GetEncryptedBeaconKeyInput_GetEncryptedBeaconKeyInput as DafnyGetEncryptedBeaconKeyInput,
+    GetEncryptedBeaconKeyOutput_GetEncryptedBeaconKeyOutput as DafnyGetEncryptedBeaconKeyOutput,
+    GetEncryptedBranchKeyVersionInput_GetEncryptedBranchKeyVersionInput as DafnyGetEncryptedBranchKeyVersionInput,
+    GetEncryptedBranchKeyVersionOutput_GetEncryptedBranchKeyVersionOutput as DafnyGetEncryptedBranchKeyVersionOutput,
+    GetKeyStorageInfoInput_GetKeyStorageInfoInput as DafnyGetKeyStorageInfoInput,
+    GetKeyStorageInfoOutput_GetKeyStorageInfoOutput as DafnyGetKeyStorageInfoOutput,
+    WriteNewEncryptedBranchKeyInput_WriteNewEncryptedBranchKeyInput as DafnyWriteNewEncryptedBranchKeyInput,
+    WriteNewEncryptedBranchKeyOutput_WriteNewEncryptedBranchKeyOutput as DafnyWriteNewEncryptedBranchKeyOutput,
+    WriteNewEncryptedBranchKeyVersionInput_WriteNewEncryptedBranchKeyVersionInput as DafnyWriteNewEncryptedBranchKeyVersionInput,
+    WriteNewEncryptedBranchKeyVersionOutput_WriteNewEncryptedBranchKeyVersionOutput as DafnyWriteNewEncryptedBranchKeyVersionOutput,
+)
+import aws_cryptographic_material_providers.internaldafny.generated.module_
+import aws_cryptographic_material_providers.smithygenerated.aws_cryptography_keystore.dafny_to_smithy
+from aws_cryptographic_material_providers.smithygenerated.aws_cryptography_keystore.errors import (
+    _smithy_error_to_dafny_error,
+)
+import aws_cryptographic_material_providers.smithygenerated.aws_cryptography_keystore.models
+import aws_cryptographic_material_providers.smithygenerated.aws_cryptography_keystore.smithy_to_dafny
+from smithy_dafny_standard_library.internaldafny.generated import Wrappers
+from typing import Any, Dict
+
+
+class IKeyStorageInterface(metaclass=abc.ABCMeta):
+
+    @classmethod
+    def __subclasshook__(cls, subclass):
+        return (
+            hasattr(subclass, "WriteNewEncryptedBranchKey")
+            and callable(subclass.WriteNewEncryptedBranchKey)
+            and hasattr(subclass, "WriteNewEncryptedBranchKeyVersion")
+            and callable(subclass.WriteNewEncryptedBranchKeyVersion)
+            and hasattr(subclass, "GetEncryptedActiveBranchKey")
+            and callable(subclass.GetEncryptedActiveBranchKey)
+            and hasattr(subclass, "GetEncryptedBranchKeyVersion")
+            and callable(subclass.GetEncryptedBranchKeyVersion)
+            and hasattr(subclass, "GetEncryptedBeaconKey")
+            and callable(subclass.GetEncryptedBeaconKey)
+            and hasattr(subclass, "GetKeyStorageInfo")
+            and callable(subclass.GetKeyStorageInfo)
+        )
+
+    @abc.abstractmethod
+    def write_new_encrypted_branch_key(
+        self,
+        param: "aws_cryptographic_material_providers.smithygenerated.aws_cryptography_keystore.models.WriteNewEncryptedBranchKeyInput",
+    ) -> "aws_cryptographic_material_providers.smithygenerated.aws_cryptography_keystore.models.WriteNewEncryptedBranchKeyOutput":
+        """WriteNewEncryptedBranchKey persists the active item, decrypt only
+        (version) item, and Beacon Key Item of a newly created Branch Key.
+        :param param: The information required to atomically write an a new
+        branch key into a key store. The identifiers for all keys passed should
+        be the same.
+
+        :returns: The output of writing a new branch key. There is
+            currently no additional information returned.
+        """
+        raise NotImplementedError
+
+    @abc.abstractmethod
+    def write_new_encrypted_branch_key_version(
+        self,
+        param: "aws_cryptographic_material_providers.smithygenerated.aws_cryptography_keystore.models.WriteNewEncryptedBranchKeyVersionInput",
+    ) -> "aws_cryptographic_material_providers.smithygenerated.aws_cryptography_keystore.models.WriteNewEncryptedBranchKeyVersionOutput":
+        """WriteNewEncryptedBranchKeyVersion persists the new active item,
+        decrypt only (version) item of a newly generated Branch Key version.
+        :param param: The information required to atomically write a new
+        version for an existing branch key into a key store. The identifiers
+        for all keys passed should be the same.
+
+        :returns: The output of writing a new version for an existing
+            branch key. There is currently no additional information
+            returned.
+        """
+        raise NotImplementedError
+
+    @abc.abstractmethod
+    def get_encrypted_active_branch_key(
+        self,
+        param: "aws_cryptographic_material_providers.smithygenerated.aws_cryptography_keystore.models.GetEncryptedActiveBranchKeyInput",
+    ) -> "aws_cryptographic_material_providers.smithygenerated.aws_cryptography_keystore.models.GetEncryptedActiveBranchKeyOutput":
+        """Get the ACTIVE branch key for encryption for an existing branch key.
+
+        :param param: Get the ACTIVE version for a particular Branch
+            Key.
+        :returns: Outputs for getting a Branch Key's ACTIVE version.
+        """
+        raise NotImplementedError
+
+    @abc.abstractmethod
+    def get_encrypted_branch_key_version(
+        self,
+        param: "aws_cryptographic_material_providers.smithygenerated.aws_cryptography_keystore.models.GetEncryptedBranchKeyVersionInput",
+    ) -> "aws_cryptographic_material_providers.smithygenerated.aws_cryptography_keystore.models.GetEncryptedBranchKeyVersionOutput":
+        """Get a specific branch key version for an existing branch key.
+
+        :param param: Inputs for getting a version of a Branch Key.
+        :returns: Outputs for getting a version of a Branch Key.
+        """
+        raise NotImplementedError
+
+    @abc.abstractmethod
+    def get_encrypted_beacon_key(
+        self,
+        param: "aws_cryptographic_material_providers.smithygenerated.aws_cryptography_keystore.models.GetEncryptedBeaconKeyInput",
+    ) -> "aws_cryptographic_material_providers.smithygenerated.aws_cryptography_keystore.models.GetEncryptedBeaconKeyOutput":
+        """Get the beacon key associated with an existing branch key.
+
+        :param param: Inputs for getting a Beacon Key
+        :returns: Outputs for getting a Beacon Key
+        """
+        raise NotImplementedError
+
+    @abc.abstractmethod
+    def get_key_storage_info(
+        self,
+        param: "aws_cryptographic_material_providers.smithygenerated.aws_cryptography_keystore.models.GetKeyStorageInfoInput",
+    ) -> "aws_cryptographic_material_providers.smithygenerated.aws_cryptography_keystore.models.GetKeyStorageInfoOutput":
+        """Gets information about the underlying storage system.
+
+        :param param: Input for getting information about the underlying
+            storage.
+        :returns: Output containing information about the underlying
+            storage.
+        """
+        raise NotImplementedError
+
+    def WriteNewEncryptedBranchKey(
+        self, dafny_input: "DafnyWriteNewEncryptedBranchKeyInput"
+    ) -> "DafnyWriteNewEncryptedBranchKeyOutput":
+        """Do not use.
+
+        This method allows custom implementations of this interface to
+        interact with generated code.
+        """
+        native_input = aws_cryptographic_material_providers.smithygenerated.aws_cryptography_keystore.dafny_to_smithy.aws_cryptography_keystore_WriteNewEncryptedBranchKeyInput(
+            dafny_input
+        )
+        try:
+            native_output = self.write_new_encrypted_branch_key(native_input)
+            dafny_output = aws_cryptographic_material_providers.smithygenerated.aws_cryptography_keystore.smithy_to_dafny.aws_cryptography_keystore_WriteNewEncryptedBranchKeyOutput(
+                native_output
+            )
+            return Wrappers.Result_Success(dafny_output)
+        except Exception as e:
+            error = _smithy_error_to_dafny_error(e)
+            return Wrappers.Result_Failure(error)
+
+    def WriteNewEncryptedBranchKeyVersion(
+        self, dafny_input: "DafnyWriteNewEncryptedBranchKeyVersionInput"
+    ) -> "DafnyWriteNewEncryptedBranchKeyVersionOutput":
+        """Do not use.
+
+        This method allows custom implementations of this interface to
+        interact with generated code.
+        """
+        native_input = aws_cryptographic_material_providers.smithygenerated.aws_cryptography_keystore.dafny_to_smithy.aws_cryptography_keystore_WriteNewEncryptedBranchKeyVersionInput(
+            dafny_input
+        )
+        try:
+            native_output = self.write_new_encrypted_branch_key_version(native_input)
+            dafny_output = aws_cryptographic_material_providers.smithygenerated.aws_cryptography_keystore.smithy_to_dafny.aws_cryptography_keystore_WriteNewEncryptedBranchKeyVersionOutput(
+                native_output
+            )
+            return Wrappers.Result_Success(dafny_output)
+        except Exception as e:
+            error = _smithy_error_to_dafny_error(e)
+            return Wrappers.Result_Failure(error)
+
+    def GetEncryptedActiveBranchKey(
+        self, dafny_input: "DafnyGetEncryptedActiveBranchKeyInput"
+    ) -> "DafnyGetEncryptedActiveBranchKeyOutput":
+        """Do not use.
+
+        This method allows custom implementations of this interface to
+        interact with generated code.
+        """
+        native_input = aws_cryptographic_material_providers.smithygenerated.aws_cryptography_keystore.dafny_to_smithy.aws_cryptography_keystore_GetEncryptedActiveBranchKeyInput(
+            dafny_input
+        )
+        try:
+            native_output = self.get_encrypted_active_branch_key(native_input)
+            dafny_output = aws_cryptographic_material_providers.smithygenerated.aws_cryptography_keystore.smithy_to_dafny.aws_cryptography_keystore_GetEncryptedActiveBranchKeyOutput(
+                native_output
+            )
+            return Wrappers.Result_Success(dafny_output)
+        except Exception as e:
+            error = _smithy_error_to_dafny_error(e)
+            return Wrappers.Result_Failure(error)
+
+    def GetEncryptedBranchKeyVersion(
+        self, dafny_input: "DafnyGetEncryptedBranchKeyVersionInput"
+    ) -> "DafnyGetEncryptedBranchKeyVersionOutput":
+        """Do not use.
+
+        This method allows custom implementations of this interface to
+        interact with generated code.
+        """
+        native_input = aws_cryptographic_material_providers.smithygenerated.aws_cryptography_keystore.dafny_to_smithy.aws_cryptography_keystore_GetEncryptedBranchKeyVersionInput(
+            dafny_input
+        )
+        try:
+            native_output = self.get_encrypted_branch_key_version(native_input)
+            dafny_output = aws_cryptographic_material_providers.smithygenerated.aws_cryptography_keystore.smithy_to_dafny.aws_cryptography_keystore_GetEncryptedBranchKeyVersionOutput(
+                native_output
+            )
+            return Wrappers.Result_Success(dafny_output)
+        except Exception as e:
+            error = _smithy_error_to_dafny_error(e)
+            return Wrappers.Result_Failure(error)
+
+    def GetEncryptedBeaconKey(
+        self, dafny_input: "DafnyGetEncryptedBeaconKeyInput"
+    ) -> "DafnyGetEncryptedBeaconKeyOutput":
+        """Do not use.
+
+        This method allows custom implementations of this interface to
+        interact with generated code.
+        """
+        native_input = aws_cryptographic_material_providers.smithygenerated.aws_cryptography_keystore.dafny_to_smithy.aws_cryptography_keystore_GetEncryptedBeaconKeyInput(
+            dafny_input
+        )
+        try:
+            native_output = self.get_encrypted_beacon_key(native_input)
+            dafny_output = aws_cryptographic_material_providers.smithygenerated.aws_cryptography_keystore.smithy_to_dafny.aws_cryptography_keystore_GetEncryptedBeaconKeyOutput(
+                native_output
+            )
+            return Wrappers.Result_Success(dafny_output)
+        except Exception as e:
+            error = _smithy_error_to_dafny_error(e)
+            return Wrappers.Result_Failure(error)
+
+    def GetKeyStorageInfo(
+        self, dafny_input: "DafnyGetKeyStorageInfoInput"
+    ) -> "DafnyGetKeyStorageInfoOutput":
+        """Do not use.
+
+        This method allows custom implementations of this interface to
+        interact with generated code.
+        """
+        native_input = aws_cryptographic_material_providers.smithygenerated.aws_cryptography_keystore.dafny_to_smithy.aws_cryptography_keystore_GetKeyStorageInfoInput(
+            dafny_input
+        )
+        try:
+            native_output = self.get_key_storage_info(native_input)
+            dafny_output = aws_cryptographic_material_providers.smithygenerated.aws_cryptography_keystore.smithy_to_dafny.aws_cryptography_keystore_GetKeyStorageInfoOutput(
+                native_output
+            )
+            return Wrappers.Result_Success(dafny_output)
+        except Exception as e:
+            error = _smithy_error_to_dafny_error(e)
+            return Wrappers.Result_Failure(error)
+
+
+class KeyStorageInterface(IKeyStorageInterface):
+
+    _impl: (
+        aws_cryptographic_material_providers.internaldafny.generated.AwsCryptographyKeyStoreTypes.IKeyStorageInterface
+    )
+
+    def __init__(
+        self,
+        _impl: aws_cryptographic_material_providers.internaldafny.generated.AwsCryptographyKeyStoreTypes.IKeyStorageInterface,
+    ):
+        self._impl = _impl
+
+    def write_new_encrypted_branch_key(
+        self,
+        param: "aws_cryptographic_material_providers.smithygenerated.aws_cryptography_keystore.models.WriteNewEncryptedBranchKeyInput",
+    ) -> "aws_cryptographic_material_providers.smithygenerated.aws_cryptography_keystore.models.WriteNewEncryptedBranchKeyOutput":
+        """WriteNewEncryptedBranchKey persists the active item, decrypt only
+        (version) item, and Beacon Key Item of a newly created Branch Key.
+        :param param: The information required to atomically write an a new
+        branch key into a key store. The identifiers for all keys passed should
+        be the same.
+
+        :returns: The output of writing a new branch key. There is
+            currently no additional information returned.
+        """
+        dafny_output = self._impl.WriteNewEncryptedBranchKey(
+            aws_cryptographic_material_providers.smithygenerated.aws_cryptography_keystore.smithy_to_dafny.aws_cryptography_keystore_WriteNewEncryptedBranchKeyInput(
+                param
+            )
+        )
+        if dafny_output.IsFailure():
+            from aws_cryptographic_material_providers.smithygenerated.aws_cryptography_keystore.deserialize import (
+                _deserialize_error as aws_cryptography_keystore_deserialize_error,
+            )
+
+            raise aws_cryptography_keystore_deserialize_error(dafny_output.error)
+
+        else:
+            return aws_cryptographic_material_providers.smithygenerated.aws_cryptography_keystore.dafny_to_smithy.aws_cryptography_keystore_WriteNewEncryptedBranchKeyOutput(
+                dafny_output.value
+            )
+
+    def write_new_encrypted_branch_key_version(
+        self,
+        param: "aws_cryptographic_material_providers.smithygenerated.aws_cryptography_keystore.models.WriteNewEncryptedBranchKeyVersionInput",
+    ) -> "aws_cryptographic_material_providers.smithygenerated.aws_cryptography_keystore.models.WriteNewEncryptedBranchKeyVersionOutput":
+        """WriteNewEncryptedBranchKeyVersion persists the new active item,
+        decrypt only (version) item of a newly generated Branch Key version.
+        :param param: The information required to atomically write a new
+        version for an existing branch key into a key store. The identifiers
+        for all keys passed should be the same.
+
+        :returns: The output of writing a new version for an existing
+            branch key. There is currently no additional information
+            returned.
+        """
+        dafny_output = self._impl.WriteNewEncryptedBranchKeyVersion(
+            aws_cryptographic_material_providers.smithygenerated.aws_cryptography_keystore.smithy_to_dafny.aws_cryptography_keystore_WriteNewEncryptedBranchKeyVersionInput(
+                param
+            )
+        )
+        if dafny_output.IsFailure():
+            from aws_cryptographic_material_providers.smithygenerated.aws_cryptography_keystore.deserialize import (
+                _deserialize_error as aws_cryptography_keystore_deserialize_error,
+            )
+
+            raise aws_cryptography_keystore_deserialize_error(dafny_output.error)
+
+        else:
+            return aws_cryptographic_material_providers.smithygenerated.aws_cryptography_keystore.dafny_to_smithy.aws_cryptography_keystore_WriteNewEncryptedBranchKeyVersionOutput(
+                dafny_output.value
+            )
+
+    def get_encrypted_active_branch_key(
+        self,
+        param: "aws_cryptographic_material_providers.smithygenerated.aws_cryptography_keystore.models.GetEncryptedActiveBranchKeyInput",
+    ) -> "aws_cryptographic_material_providers.smithygenerated.aws_cryptography_keystore.models.GetEncryptedActiveBranchKeyOutput":
+        """Get the ACTIVE branch key for encryption for an existing branch key.
+
+        :param param: Get the ACTIVE version for a particular Branch
+            Key.
+        :returns: Outputs for getting a Branch Key's ACTIVE version.
+        """
+        dafny_output = self._impl.GetEncryptedActiveBranchKey(
+            aws_cryptographic_material_providers.smithygenerated.aws_cryptography_keystore.smithy_to_dafny.aws_cryptography_keystore_GetEncryptedActiveBranchKeyInput(
+                param
+            )
+        )
+        if dafny_output.IsFailure():
+            from aws_cryptographic_material_providers.smithygenerated.aws_cryptography_keystore.deserialize import (
+                _deserialize_error as aws_cryptography_keystore_deserialize_error,
+            )
+
+            raise aws_cryptography_keystore_deserialize_error(dafny_output.error)
+
+        else:
+            return aws_cryptographic_material_providers.smithygenerated.aws_cryptography_keystore.dafny_to_smithy.aws_cryptography_keystore_GetEncryptedActiveBranchKeyOutput(
+                dafny_output.value
+            )
+
+    def get_encrypted_branch_key_version(
+        self,
+        param: "aws_cryptographic_material_providers.smithygenerated.aws_cryptography_keystore.models.GetEncryptedBranchKeyVersionInput",
+    ) -> "aws_cryptographic_material_providers.smithygenerated.aws_cryptography_keystore.models.GetEncryptedBranchKeyVersionOutput":
+        """Get a specific branch key version for an existing branch key.
+
+        :param param: Inputs for getting a version of a Branch Key.
+        :returns: Outputs for getting a version of a Branch Key.
+        """
+        dafny_output = self._impl.GetEncryptedBranchKeyVersion(
+            aws_cryptographic_material_providers.smithygenerated.aws_cryptography_keystore.smithy_to_dafny.aws_cryptography_keystore_GetEncryptedBranchKeyVersionInput(
+                param
+            )
+        )
+        if dafny_output.IsFailure():
+            from aws_cryptographic_material_providers.smithygenerated.aws_cryptography_keystore.deserialize import (
+                _deserialize_error as aws_cryptography_keystore_deserialize_error,
+            )
+
+            raise aws_cryptography_keystore_deserialize_error(dafny_output.error)
+
+        else:
+            return aws_cryptographic_material_providers.smithygenerated.aws_cryptography_keystore.dafny_to_smithy.aws_cryptography_keystore_GetEncryptedBranchKeyVersionOutput(
+                dafny_output.value
+            )
+
+    def get_encrypted_beacon_key(
+        self,
+        param: "aws_cryptographic_material_providers.smithygenerated.aws_cryptography_keystore.models.GetEncryptedBeaconKeyInput",
+    ) -> "aws_cryptographic_material_providers.smithygenerated.aws_cryptography_keystore.models.GetEncryptedBeaconKeyOutput":
+        """Get the beacon key associated with an existing branch key.
+
+        :param param: Inputs for getting a Beacon Key
+        :returns: Outputs for getting a Beacon Key
+        """
+        dafny_output = self._impl.GetEncryptedBeaconKey(
+            aws_cryptographic_material_providers.smithygenerated.aws_cryptography_keystore.smithy_to_dafny.aws_cryptography_keystore_GetEncryptedBeaconKeyInput(
+                param
+            )
+        )
+        if dafny_output.IsFailure():
+            from aws_cryptographic_material_providers.smithygenerated.aws_cryptography_keystore.deserialize import (
+                _deserialize_error as aws_cryptography_keystore_deserialize_error,
+            )
+
+            raise aws_cryptography_keystore_deserialize_error(dafny_output.error)
+
+        else:
+            return aws_cryptographic_material_providers.smithygenerated.aws_cryptography_keystore.dafny_to_smithy.aws_cryptography_keystore_GetEncryptedBeaconKeyOutput(
+                dafny_output.value
+            )
+
+    def get_key_storage_info(
+        self,
+        param: "aws_cryptographic_material_providers.smithygenerated.aws_cryptography_keystore.models.GetKeyStorageInfoInput",
+    ) -> "aws_cryptographic_material_providers.smithygenerated.aws_cryptography_keystore.models.GetKeyStorageInfoOutput":
+        """Gets information about the underlying storage system.
+
+        :param param: Input for getting information about the underlying
+            storage.
+        :returns: Output containing information about the underlying
+            storage.
+        """
+        dafny_output = self._impl.GetKeyStorageInfo(
+            aws_cryptographic_material_providers.smithygenerated.aws_cryptography_keystore.smithy_to_dafny.aws_cryptography_keystore_GetKeyStorageInfoInput(
+                param
+            )
+        )
+        if dafny_output.IsFailure():
+            from aws_cryptographic_material_providers.smithygenerated.aws_cryptography_keystore.deserialize import (
+                _deserialize_error as aws_cryptography_keystore_deserialize_error,
+            )
+
+            raise aws_cryptography_keystore_deserialize_error(dafny_output.error)
+
+        else:
+            return aws_cryptographic_material_providers.smithygenerated.aws_cryptography_keystore.dafny_to_smithy.aws_cryptography_keystore_GetKeyStorageInfoOutput(
+                dafny_output.value
+            )
+
+    @staticmethod
+    def from_dict(d: Dict[str, Any]) -> "KeyStorageInterface":
+        return KeyStorageInterface(d["_impl"])
+
+    def as_dict(self) -> Dict[str, Any]:
+        return {"_impl": self._impl}
