AwsCryptographicMaterialProviders/dafny/AwsCryptographyKeyStore/test/TestCreateKeys.dfy
@@ -3,10 +3,9 @@
 
 include "../src/Index.dfy"
 include "Fixtures.dfy"
-include "../src/Structure.dfy"
 include "CleanupItems.dfy"
 
-module TestCreateKeys {
+module {:options "/functionSyntax:4" } TestCreateKeys {
   import Types = AwsCryptographyKeyStoreTypes
   import ComAmazonawsKmsTypes
   import KMS = Com.Amazonaws.Kms
@@ -14,11 +13,13 @@ module TestCreateKeys {
   import KeyStore
   import opened Wrappers
   import opened Fixtures
-  import Structure
   import UTF8
   import CleanupItems
-  import DDBKeystoreOperations
+  import Structure
+  import DefaultKeyStorageInterface
+  import KmsArn
   import UUID
+  import AwsArnParsing
 
   /*
     // If you need to re-create the MRK Branch Keys
@@ -73,10 +74,17 @@ module TestCreateKeys {
       id := None,
       kmsConfiguration := kmsConfig,
       logicalKeyStoreName := logicalKeyStoreName,
-      grantTokens := None,
-      ddbTableName := branchKeyStoreName,
-      ddbClient := Some(ddbClient),
-      kmsClient := Some(kmsClient)
+      storage := Some(
+        Types.ddb(
+          Types.DynamoDBTable(
+            ddbTableName := branchKeyStoreName,
+            ddbClient := Some(ddbClient)
+          ))),
+      keyManagement := Some(
+        Types.kms(
+          Types.AwsKms(
+            kmsClient := Some(kmsClient)
+          )))
     );
 
     var keyStore :- expect KeyStore.KeyStore(keyStoreConfig);
@@ -101,6 +109,32 @@ module TestCreateKeys {
         branchKeyIdentifier := branchKeyId.branchKeyIdentifier,
         branchKeyVersion := branchKeyVersion
       ));
+
+    var encryptedActive :- expect keyStore.config.storage.GetEncryptedActiveBranchKey(
+      Types.GetEncryptedActiveBranchKeyInput(
+        Identifier := branchKeyId.branchKeyIdentifier
+      )
+    );
+
+    var encryptedVersion :- expect keyStore.config.storage.GetEncryptedBranchKeyVersion(
+      Types.GetEncryptedBranchKeyVersionInput(
+        Identifier := branchKeyId.branchKeyIdentifier,
+        Version := encryptedActive.Item.Type.ActiveHierarchicalSymmetricVersion.Version
+      )
+    );
+
+    var encryptedBeacon :- expect keyStore.config.storage.GetEncryptedBeaconKey(
+      Types.GetEncryptedBeaconKeyInput(
+        Identifier := branchKeyId.branchKeyIdentifier
+      )
+    );
+
+    //= aws-encryption-sdk-specification/framework/branch-key-store.md#branch-key-and-beacon-key-creation
+    //= type=test
+    //# This timestamp MUST be in ISO 8601 format in UTC, to microsecond precision (e.g. “YYYY-MM-DDTHH:mm:ss.ssssssZ“)
+    expect ISO8601?(encryptedActive.Item.CreateTime);
+    expect ISO8601?(encryptedVersion.Item.CreateTime);
+    expect ISO8601?(encryptedBeacon.Item.CreateTime);
 
     // Since this process uses a read DDB table,
     // the number of records will forever increase.
@@ -137,6 +171,26 @@ module TestCreateKeys {
 
   }
 
+  lemma ISO8601Test()
+  {
+    assert ISO8601?("2024-08-06T17:23:25.000874Z");
+  }
+
+  predicate ISO8601?(
+    CreateTime: string
+  )
+  {
+    // “YYYY-MM-DDTHH:mm:ss.ssssssZ“
+    && |CreateTime| == 27
+    && CreateTime[4] == '-'
+    && CreateTime[7] == '-'
+    && CreateTime[10] == 'T'
+    && CreateTime[13] == ':'
+    && CreateTime[16] == ':'
+    && CreateTime[19] == '.'
+    && CreateTime[26] == 'Z'
+  }
+
   method {:test} TestCreateOptions()
   {
     var kmsClient :- expect KMS.KMSClient();
@@ -147,10 +201,17 @@ module TestCreateKeys {
       id := None,
       kmsConfiguration := kmsConfig,
       logicalKeyStoreName := logicalKeyStoreName,
-      grantTokens := None,
-      ddbTableName := branchKeyStoreName,
-      ddbClient := Some(ddbClient),
-      kmsClient := Some(kmsClient)
+      storage := Some(
+        Types.ddb(
+          Types.DynamoDBTable(
+            ddbTableName := branchKeyStoreName,
+            ddbClient := Some(ddbClient)
+          ))),
+      keyManagement := Some(
+        Types.kms(
+          Types.AwsKms(
+            kmsClient := Some(kmsClient)
+          )))
     );
 
     var keyStore :- expect KeyStore.KeyStore(keyStoreConfig);
@@ -214,26 +275,41 @@ module TestCreateKeys {
       id := None,
       kmsConfiguration := kmsConfig,
       logicalKeyStoreName := logicalKeyStoreName,
-      grantTokens := None,
-      ddbTableName := branchKeyStoreName,
-      ddbClient := Some(ddbClient),
-      kmsClient := Some(kmsClient)
+      storage := Some(
+        Types.ddb(
+          Types.DynamoDBTable(
+            ddbTableName := branchKeyStoreName,
+            ddbClient := Some(ddbClient)
+          ))),
+      keyManagement := Some(
+        Types.kms(
+          Types.AwsKms(
+            kmsClient := Some(kmsClient)
+          )))
     );
 
     var keyStore :- expect KeyStore.KeyStore(keyStoreConfig);
 
-    var attempt := keyStore.CreateKey(Types.CreateKeyInput(
-                                        branchKeyIdentifier := Some(branchKeyId),
-                                        encryptionContext := None
-                                      ));
+    var attempt := keyStore.CreateKey(
+      Types.CreateKeyInput(
+        branchKeyIdentifier := Some(branchKeyId),
+        encryptionContext := None
+      ));
 
     expect attempt.Failure?;
   }
 
   method {:test} InsertingADuplicateWillFail()
   {
-    assume {:axiom} false;
     var ddbClient :- expect DDB.DynamoDBClient();
+    var customEC := map[];
+
+    expect 0 < |branchKeyId|;
+    expect 0 < |branchKeyIdActiveVersion|;
+    expect forall k <- customEC :: DDB.Types.IsValid_AttributeName(Structure.ENCRYPTION_CONTEXT_PREFIX + k);
+    expect KMS.Types.IsValid_KeyIdType(keyArn);
+    expect AwsArnParsing.ParseAwsKmsArn(keyArn).Success?;
+    expect KmsArn.ValidKmsArn?(keyArn);
 
     var encryptionContext := Structure.DecryptOnlyBranchKeyEncryptionContext(
       branchKeyId,
@@ -241,15 +317,25 @@ module TestCreateKeys {
       "",
       "",
       keyArn,
-      map[]
+      customEC
+    );
+    var ddbTableNameUtf8 :- expect UTF8.Encode(branchKeyStoreName);
+    var logicalKeyStoreNameUtf8 :- expect UTF8.Encode("");
+
+    var storage := new DefaultKeyStorageInterface.DynamoDBKeyStorageInterface(
+      ddbTableName := branchKeyStoreName,
+      ddbClient := ddbClient,
+      logicalKeyStoreName := "",
+      ddbTableNameUtf8 := ddbTableNameUtf8,
+      logicalKeyStoreNameUtf8 := logicalKeyStoreNameUtf8
     );
 
-    var output := DDBKeystoreOperations.WriteNewKeyToStore(
-      Structure.ToAttributeMap(encryptionContext, [1]),
-      Structure.ToAttributeMap(Structure.ActiveBranchKeyEncryptionContext(encryptionContext), [2]),
-      Structure.ToAttributeMap(Structure.BeaconKeyEncryptionContext(encryptionContext), [3]),
-      branchKeyStoreName,
-      ddbClient
+    var output := storage.WriteNewEncryptedBranchKey(
+      Types.WriteNewEncryptedBranchKeyInput(
+        Version := Structure.ConstructEncryptedHierarchicalKey(encryptionContext, [1]),
+        Active := Structure.ConstructEncryptedHierarchicalKey(Structure.ActiveBranchKeyEncryptionContext(encryptionContext), [2]),
+        Beacon := Structure.ConstructEncryptedHierarchicalKey(Structure.BeaconKeyEncryptionContext(encryptionContext), [2])
+      )
     );
 
     expect output.Failure?;
@@ -257,8 +343,15 @@ module TestCreateKeys {
 
   method {:test} InsertingADuplicateWillWithADifferentVersionFail()
   {
-    assume {:axiom} false;
     var ddbClient :- expect DDB.DynamoDBClient();
+    var customEC := map[];
+
+    expect 0 < |branchKeyId|;
+    expect 0 < |branchKeyIdActiveVersion|;
+    expect forall k <- customEC :: DDB.Types.IsValid_AttributeName(Structure.ENCRYPTION_CONTEXT_PREFIX + k);
+    expect KMS.Types.IsValid_KeyIdType(keyArn);
+    expect AwsArnParsing.ParseAwsKmsArn(keyArn).Success?;
+    expect KmsArn.ValidKmsArn?(keyArn);
 
     var encryptionContext := Structure.DecryptOnlyBranchKeyEncryptionContext(
       branchKeyId,
@@ -266,15 +359,25 @@ module TestCreateKeys {
       "",
       "",
       keyArn,
-      map[]
+      customEC
+    );
+    var ddbTableNameUtf8 :- expect UTF8.Encode(branchKeyStoreName);
+    var logicalKeyStoreNameUtf8 :- expect UTF8.Encode("");
+
+    var storage := new DefaultKeyStorageInterface.DynamoDBKeyStorageInterface(
+      ddbTableName := branchKeyStoreName,
+      ddbClient := ddbClient,
+      logicalKeyStoreName := "",
+      ddbTableNameUtf8 := ddbTableNameUtf8,
+      logicalKeyStoreNameUtf8 := logicalKeyStoreNameUtf8
     );
 
-    var output := DDBKeystoreOperations.WriteNewKeyToStore(
-      Structure.ToAttributeMap(encryptionContext, [1]),
-      Structure.ToAttributeMap(Structure.ActiveBranchKeyEncryptionContext(encryptionContext), [2]),
-      Structure.ToAttributeMap(Structure.BeaconKeyEncryptionContext(encryptionContext), [3]),
-      branchKeyStoreName,
-      ddbClient
+    var output := storage.WriteNewEncryptedBranchKey(
+      Types.WriteNewEncryptedBranchKeyInput(
+        Version := Structure.ConstructEncryptedHierarchicalKey(encryptionContext, [1]),
+        Active := Structure.ConstructEncryptedHierarchicalKey(Structure.ActiveBranchKeyEncryptionContext(encryptionContext), [2]),
+        Beacon := Structure.ConstructEncryptedHierarchicalKey(Structure.BeaconKeyEncryptionContext(encryptionContext), [2])
+      )
     );
 
     expect output.Failure?;
